draft of Multihash and Cid

Ipld/UnsignedVarint.lean
@@ -1,36 +1,40 @@
 import Ipld.Utils
 
-def toVarIntCore : Nat → Nat → ByteArray → ByteArray
-| 0, n, bytes => bytes
-| fuel+1, n, bytes =>
-      let b: UInt8 := UInt8.ofNat (n % 128);
-      let n' := n / 128;
-      if n' = 0 then (bytes.push b)
-      else toVarIntCore fuel n' (bytes.push (b + 128))
+def toVarIntCore : Nat → Nat → List UInt8
+| 0, n => []
+| fuel+1, n =>
+  let b: UInt8 := UInt8.ofNat (n % 128);
+  let n' := n / 128;
+  if n' = 0 then [b]
+  else (b + 128) :: (toVarIntCore fuel n')
 
-def toVarInt (n: Nat) : ByteArray := 
-  toVarIntCore (n+1) n { data := #[] }
+def toVarInt (n: Nat) : List UInt8 := 
+  toVarIntCore (n+1) n 
 
-def fromVarInt (b: ByteArray) : Nat := do
-  let mut x := 0
-  for i in [:b.size] do
-    x := x + Nat.shiftLeft (UInt8.toNat b.data[i] % 128) (i * 7)
-  return x
+def readVarIntCore : Nat → Nat → List UInt8 → Nat → Option (Nat × List UInt8)
+| 0, i, bs, n => some (n, bs)
+| fuel+1, i, [], n => none
+| fuel+1, i, b::bs, n => 
+  let b' := Nat.shiftLeft (UInt8.toNat b % 128) (i * 7)
+  if b / 128 == 0 then (n + b', bs) else readVarIntCore fuel (i + 1) bs (n + b')
+
+def readVarInt (b: List UInt8) : Option (Nat × List UInt8) :=
+  readVarIntCore b.length 0 b 0
 
 instance : BEq ByteArray where
   beq a b := a.data == b.data
 
---#eval fromVarInt (toVarInt 1) == 1
---#eval (toVarInt 127) == { data := #[0b01111111] }
---
---#reduce fromVarInt (toVarInt 1) = 1 
---
---#eval fromVarInt (toVarInt 127) == 127
---#eval toVarInt 255 
---#eval (toVarInt 255 == { data := #[0b11111111, 0b00000001] })
---#eval (toVarInt 255 == { data := #[0b01111111, 0b00000001] })
---#eval fromVarInt (toVarInt 255) == 255
---#eval (toVarInt 300 == { data := #[0b10101100, 0b00000010] })
---#eval fromVarInt (toVarInt 300) == 300
---#eval (toVarInt 16384 == { data := #[0b10000000, 0b10000000, 0b00000001] })
---#eval fromVarInt (toVarInt 16384) == 16384
+
+namespace Test
+
+theorem encode1 : toVarInt 1 = [0b00000001] := rfl
+theorem read1 : readVarInt  [0b00000001] = some (1, []) := rfl
+theorem encode127 : toVarInt 127 =  [0b01111111] := rfl
+theorem read127 : readVarInt  [0b01111111] = some (127, []) := rfl
+theorem encode128 : toVarInt 128 =  [0b10000000, 0b00000001] := rfl
+theorem read128 : readVarInt  [0b10000000, 0b00000001] = some (128, []) := rfl
+theorem encode300 : toVarInt 300 =  [0b10101100, 0b00000010] := rfl
+theorem read300 : readVarInt  [0b10101100, 0b00000010] = some (300, []) := rfl
+theorem encode16384 : toVarInt 16384 =  [0b10000000, 0b10000000, 0b00000001] := rfl
+theorem read16384 : readVarInt  [0b10000000, 0b10000000, 0b00000001] = some (16384, []) := rfl
+end Test
