Ipld/Cid.lean
@@ -1,7 +1,37 @@
 import Ipld.Multihash
+import Ipld.Multibase
 
 structure Cid where
   version : Nat
   codec: Nat
   hash: Multihash
   deriving Inhabited
+
+namespace Cid
+def toBytes (self : Cid) : List UInt8 :=
+ (toVarInt self.version) ++ (toVarInt self.codec) ++ Multihash.toBytes self.hash
+
+def toString (self: Cid) : String :=
+  Multibase.encode Multibase.Base32 (toBytes self)
+
+instance : ToString Cid where
+  toString := toString
+
+def fromBytes (bytes : List UInt8) : Option Cid :=
+  Option.bind (readVarInt bytes) $ fun (version, bytes) =>
+  Option.bind (readVarInt bytes) $ fun (codec, bytes) =>
+  Option.bind (Multihash.fromBytes bytes) $ fun hash =>
+  some { version, codec, hash}
+
+namespace Test
+
+def ex1 : Cid := { version := 0x1, codec := 0x11, hash := Multihash.Test.ex1 }
+
+#eval ex1
+#eval toBytes ex1
+#eval fromBytes (toBytes ex1)
+
+
+end Test
+
+end Cid
