Ipld/Multihash.lean
@@ -1,45 +1,39 @@
 import Ipld.UnsignedVarint
+import Ipld.Multibase
 
 structure Multihash where
   code : Nat
   size : Nat
-  digest : ByteArray
+  digest : List UInt8
   deriving BEq, Inhabited
+
+
 
 namespace Multihash
 
-def toBytes (self : Multihash) : ByteArray :=
-  ByteArray.append (toVarInt self.code) $
-  ByteArray.append (toVarInt self.size) $
-  self.digest
+def toBytes (self : Multihash) : List UInt8 :=
+  (toVarInt self.code) ++ (toVarInt self.size) ++ self.digest
 
-inductive Error
-| BadDigestSize (x: Nat) (y: Nat)
-deriving BEq
+def toString (self: Multihash) : String :=
+  Multibase.encode Multibase.Base64 (toBytes self)
 
-instance [BEq ε] [BEq α] : BEq (Except ε α) where
-  beq a b := match a, b with
-  | Except.ok a, Except.ok b => a == b
-  | Except.error a, Except.error b => a == b
-  | _, _ => false
+instance : ToString Multihash where
+  toString := toString
 
-def fromBytes (bytes : ByteArray) : Except Error Multihash := do
-  let code := fromVarInt ( { data := bytes.data[0:1].toArray })
-  let size := fromVarInt ( { data := bytes.data[1:2].toArray })
-  let digest := { data := bytes.data[2:].toArray }
-  if bytes.data.size > size + 2 
-  then Except.error (Error.BadDigestSize bytes.data.size size) 
-  else return { code := code, size := size, digest := digest }
+def fromBytes (bytes : List UInt8) : Option Multihash :=
+  Option.bind (readVarInt bytes) $ fun (code, bytes) =>
+  Option.bind (readVarInt bytes) $ fun (size, bytes) =>
+  let digest := bytes
+  if digest.length > size then none
+  else some { code := code, size := size, digest := digest }
 
+namespace Test
 
-private def example1 : Multihash := { code := 0x11, size := 0x4,  digest := { data := #[0b10110110, 0b11111000, 0b01011100, 0b10110101]}}
+def ex1 : Multihash := { code := 0x11, size := 0x4,  digest := [0b10110110, 0b11111000, 0b01011100, 0b10110101]}
 
-#eval 0b101101100
-#eval (toBytes example1) 
-#eval #[0b00010001, 0b00000100, 0b10110110, 0b11111000, 0b01011100, 0b10110101]
+#eval ex1
+#eval toBytes ex1
+#eval fromBytes (toBytes ex1)
 
-#eval (toBytes example1) == { data := #[0b0001001, 0b00000100, 0b10110110, 0b11111000, 0b01011100, 0b10110101] }
-
-#eval (pure example1) == fromBytes (toBytes example1)
-
+end Test
 end Multihash
